Modular public-key signature and EF-CMA theories.
Towards a module-based formalization of PSS (with sanity check).

examples/PSS.ec
@@ -1,143 +1,47 @@
-require import RandOrcl.
-require import Array.
 require import Bitstring.
-require import Map.
-require import FSet.
 require import Int.
 require import Distr.
-require import Bool.
 
-theory SignatureScheme.
-
-  type pkey.
-  type skey.
-
-  module type SigScheme_ROM = {
-    fun init(): unit (* This is unfortunate, but the ROM needs to be initialized *)
-    fun h(x:bitstring): bitstring
-    fun keygen(): (pkey * skey)
-    fun sign(sk:skey, m:bitstring): bitstring
-    fun verify(pk:pkey, m:bitstring, s:bitstring): bool
-  }.
-
-  op qH:int.
-  op qS:int.
-
-  module type SigScheme_Oracles_ROM = {
-    fun init(): pkey
-    fun wasQueried(m:bitstring): bool
-    fun h(x:bitstring): bitstring
-    fun sign(m:bitstring): bitstring
-    fun verify(pk:pkey, m:bitstring, s:bitstring): bool (* In theory, we don't give this one to the adversary. Check with P-Y for bug in functor application *)
-  }.
-
-  module Sig_Oracles_ROM(S:SigScheme_ROM): SigScheme_Oracles_ROM = {
-    var qs:bitstring set
-    var cH:int
-    var cS:int
-    var sk:skey
-
-    fun init():pkey = {
-      var pk:pkey;
-      S.init();
-      (pk,sk)  = S.keygen();
-      return pk; }
-
-    fun wasQueried(m:bitstring):bool = { return mem m qs; }
-
-    fun h(x:bitstring):bitstring = {
-      var r:bitstring = zeros(0);
-      if (cH < qH)
-      {
-        cH = cH + 1;
-        r  = S.h(x);
-      }
-      return r;
-    }
-
-    fun sign(m:bitstring):bitstring = {
-      var r:bitstring = zeros(0);
-      if (cS < qS)
-      {
-        cS = cS + 1;
-        qs = add m qs;
-        r  = S.sign(sk,m);
-      }
-      return r;
-    }
-
-    fun verify(pk:pkey, m:bitstring, s:bitstring):bool = {
-      var b:bool;
-      b  = S.verify(pk,m,s);
-      return b;
-    }
-  }.
-
-  module type SigAdversary_ROM(Sig:SigScheme_Oracles_ROM) = {
-    fun a(pk:pkey): (bitstring * bitstring)
-  }.
-
-  module EF_CMA(S:SigScheme_ROM, Adv:SigAdversary_ROM) = {
-    module O = Sig_Oracles_ROM(S)
-    module A = Adv(O)
-
-    fun main(): bool = {
-      var pk:pkey;
-      var m:bitstring;
-      var s:bitstring;
-      var forged:bool;
-      var queried:bool;
-      pk  = O.init();
-      (m,s)  = A.a(pk);
-      forged  = O.verify(pk,m,s);
-      queried  = O.wasQueried(m);
-      return forged /\ !queried;
-    }
-  }.
-
-(* Note: This is not necessarily the standard, this is PSS as presented in Coron 2006 (or something). *)
+(* Protocol-specific constants *)
 op k:int.
+axiom leq0_k: 0 <= k.
 op k0:int.
+axiom leq0_k0: 0 <= k0.
 op k1:int.
+axiom leq0_k1: 0 <= k1.
+axiom constraints:
+  0 <= k - k1 - 1.
+
+(* General definitions *)
+require        EF_CMA.
+
+clone import EF_CMA.EF_CMA_2ROM as PSS_EF_CMA with
+  type PKS.message <- bitstring,
+  type PKS.signature <- bitstring,
+  type PKS.Gt.from <- bitstring,
+  type PKS.Gt.to <- bitstring,
+  op PKS.Gt.dsample = Dbitstring.dbitstring (k - k1  -1),
+  type PKS.Ht.from <- bitstring,
+  type PKS.Ht.to <- bitstring,
+  op PKS.Ht.dsample = Dbitstring.dbitstring k1.
+import PKS.
 
 op keypairs: (pkey * skey) distr.
+axiom keypairsL: weight keypairs = 1%r.
+
 op rsa: pkey -> bitstring -> bitstring.
 op rsa': skey -> bitstring -> bitstring.
 
-module PSS:SigScheme_ROM = {
-  (* H *)
-  var mH:(bitstring,bitstring) map
-  fun h(x:bitstring): bitstring = {
-    var r:bitstring;
-    r = $Dbitstring.dbitstring(k1);
-    if (!in_dom x mH) mH = mH.[x <- r];
-    return proj mH.[x]; (* Yurk. We need to deal with this *)
-  }
-
-  (* G *)
-  var mG:(bitstring,bitstring) map
-  fun g(x:bitstring):bitstring = {
-    var r:bitstring;
-    r = $Dbitstring.dbitstring(k - k1 - 1);
-    if (!in_dom x mG) mG = mG.[x <- r];
-    return proj mG.[x];
-  }
-
-  (* init *)
-  fun init(): unit = {
-    mG = Map.empty;
-    mH = Map.empty;
-  }
-
+module PSS(G:Gt.Oracle,H:Ht.Oracle): Scheme = {
   fun g1(x:bitstring):bitstring = {
     var r:bitstring;
-    r  = g(x);
+    r  = G.o(x);
     return sub r 0 k0;
   }
 
   fun g2(x:bitstring):bitstring = {
     var r:bitstring;
-    r  = g(x);
+    r  = G.o(x);
     return sub r k0 (k - k0 - k1 - 1);
   }
 
@@ -158,7 +62,7 @@ module PSS:SigScheme_ROM = {
     var y:bitstring;
 
     r = $Dbitstring.dbitstring(k0);
-    w  = h(m || r);
+    w  = H.o(m || r);
     rMask  = g1(w);
     maskedR = rMask ^^ r;
     gamma  = g2(w);
@@ -177,6 +81,7 @@ module PSS:SigScheme_ROM = {
     var rMask:bitstring;
     var r:bitstring;
     var b:bool;
+
     y = (rsa pk s);
     b = y.[0];
     w = sub y 1 k1;
@@ -184,10 +89,76 @@ module PSS:SigScheme_ROM = {
     gamma = sub y (k1 + k0 + 1) (k - k1 - k0 - 1);
     rMask  = g1(w);
     r = rMask ^^ maskedR;
-    w'  = h(m || r);
+    w'  = H.o(m || r);
     gamma'  = g2(w);
     return (w = w' /\ gamma = gamma' /\ !b);
   }
 }.
 
-module PSS_Oracles = Sig_Oracles_ROM(PSS).
+module G = Gt.ROM.RO.
+module G' = Gt.WRO_Set.ARO(G).
+module H = Ht.ROM.RO.
+module H' = Ht.WRO_Set.ARO(H).
+
+section.
+declare module A:CMA {G', H', Wrap}.
+axiom losslessA (G <: Gt.ARO{A}) (H <: Ht.ARO{A}) (O <: Oracles{A}):
+  islossless O.sign => islossless H.o => islossless G.o =>
+  islossless A(G, H, O).a.
+
+module PSS_bits = PSS(G,H).
+module PSS_bors = Wrap(G,H,PSS_bits).
+module Initial = EF_CMA(G,H,PSS_bits,A).
+
+lemma terminates: islossless Initial.main.
+proof strict.
+fun.
+call (_: true ==> true);
+  first by fun.
+call (_: true ==> true); first fun.
+  call (_: true ==> true);
+    first by fun; call (_: true ==> true)=> //;
+               apply Gt.ROM.lossless_o;
+               rewrite -/(weight Gt.dsample) /Gt.dsample Dbitstring.weight_pos; smt.
+  call (_: true ==> true);
+    first by apply Ht.ROM.lossless_o;
+             rewrite -/(weight Ht.dsample) /Ht.dsample Dbitstring.weight_pos; smt.
+  wp; call (_: true ==> true);
+    first by fun; call (_: true ==> true)=> //;
+               apply Gt.ROM.lossless_o;
+               rewrite -/(weight Gt.dsample) /Gt.dsample Dbitstring.weight_pos; smt.
+  wp=> //.
+call (_: true ==> true).
+  fun true=> //.
+    by intros=> G0 H0 O; apply (losslessA G0 H0 O).
+    fun; call (_: true ==> true).
+      fun; wp; call (_: true ==> true)=> //;
+          first by fun; call (_: true ==> true)=> //;
+                     apply Gt.ROM.lossless_o=> //;
+                     rewrite -/(weight Gt.dsample) /Gt.dsample Dbitstring.weight_pos; smt.
+        wp; call (_: true ==> true)=> //;
+          first by fun; call (_: true ==> true)=> //;
+                     apply Gt.ROM.lossless_o=> //;
+                     rewrite -/(weight Gt.dsample) /Gt.dsample Dbitstring.weight_pos; smt.
+        call (_: true ==> true)=> //;
+          first by apply Ht.ROM.lossless_o=> //;
+                   rewrite -/(weight Ht.dsample) /Ht.dsample Dbitstring.weight_pos; smt.
+        by rnd=> // _; rewrite -/cpTrue -/(weight (Bitstring.Dbitstring.dbitstring k0))
+                               Bitstring.Dbitstring.weight_pos // leq0_k0.
+      wp=> //.
+    fun; if; try wp=> //.
+      call (_: true ==> true); try wp=> //;
+        first by apply Ht.ROM.lossless_o=> //;
+                 rewrite -/(weight Ht.dsample) /Ht.dsample Dbitstring.weight_pos; smt.
+    fun; if; try wp=> //.
+      call (_: true ==> true); try wp=> //;
+        first by apply Gt.ROM.lossless_o=> //;
+                 rewrite -/(weight Gt.dsample) /Gt.dsample Dbitstring.weight_pos; smt.
+call (_: true ==> true)=> //; fun;
+  call (_: true ==> true);
+    first fun; rnd=> // _; apply keypairsL.
+  wp; call (_: true ==> true);
+    first apply Gt.ROM.lossless_init.
+  wp; call (_: true ==> true)=> //;
+    apply Ht.ROM.lossless_init.
+qed.
