theories/PKS.ec
@@ -1,0 +1,130 @@
+(* Definitions for Public-Key Signatures Schemes *)
+require import FSet.
+
+theory PKS.
+  type pkey.
+  type skey.
+  type message.
+  type signature.
+
+  module type Scheme = {
+    fun keygen(): (pkey * skey)
+    fun sign(sk:skey, m:message): signature
+    fun verify(pk:pkey, m:message, s:signature): bool
+  }.
+
+  module type Oracles = { fun sign(m:message): signature }.
+
+  module Wrap(S:Scheme): Oracles = {
+    var qs: message set
+    var pk: pkey
+    var sk: skey
+
+    fun init(): pkey = {
+      qs = empty;
+      (pk,sk) = S.keygen();
+      return pk;
+    }
+
+    fun sign(m:message): signature = {
+      var s:signature;
+      qs = add m qs;
+      s = S.sign(sk,m);
+      return s;
+    }
+
+    fun fresh(m:message): bool = {
+      return !mem m qs;
+    }
+  }.
+end PKS.
+
+theory PKS_ROM.
+  type pkey.
+  type skey.
+  type message.
+  type signature.
+
+  require        RandOrcl.
+    clone import RandOrcl.
+
+  module type Scheme = {
+    fun keygen(): (pkey * skey)
+    fun sign(sk:skey, m:message): signature
+    fun verify(pk:pkey, m:message, s:signature): bool
+  }.
+
+  module type Oracles = {
+    fun sign(m:message): signature
+  }.
+
+  module Wrap(H:Oracle,S:Scheme): Oracles = {
+    var qs: message set
+    var pk: pkey
+    var sk: skey
+
+    fun init(): pkey = {
+      H.init();
+      qs = empty;
+      (pk,sk) = S.keygen();
+      return pk;
+    }
+
+    fun sign(m:message): signature = {
+      var s:signature;
+      qs = add m qs;
+      s = S.sign(sk,m);
+      return s;
+    }
+
+    fun fresh(m:message): bool = {
+      return !mem m qs;
+    }
+  }.
+end PKS_ROM.
+
+theory PKS_2ROM.
+  type pkey.
+  type skey.
+  type message.
+  type signature.
+
+  require        RandOrcl.
+    clone RandOrcl as Gt.
+    clone RandOrcl as Ht.
+
+  module type Scheme = {
+    fun keygen(): (pkey * skey)
+    fun sign(sk:skey, m:message): signature
+    fun verify(pk:pkey, m:message, s:signature): bool
+  }.
+
+  module type Oracles = {
+    fun sign(m:message): signature
+  }.
+
+  module Wrap(G:Gt.Oracle,H:Ht.Oracle,S:Scheme): Oracles = {
+    var qs: message set
+    var pk: pkey
+    var sk: skey
+
+    fun init(): pkey = {
+      H.init();
+      G.init();
+      qs = empty;
+      (pk,sk) = S.keygen();
+      return pk;
+    }
+
+    fun sign(m:message): signature = {
+      var s:signature;
+      qs = add m qs;
+      s = S.sign(sk,m);
+      return s;
+    }
+
+    fun fresh(m:message): bool = {
+      return !mem m qs;
+    }
+  }.
+end PKS_2ROM.
